inductive_proof/PN_counter/App.fst
@@ -48,6 +48,12 @@ let concrete_merge (lca s1 s2:concrete_st)
          (ensures (fun _ -> True)) =
   s1 + s2 - lca
 
+let merge_is_comm (lca s1 s2:st)
+  : Lemma (requires consistent_branches lca s1 s2 /\
+                    (exists l1 l2. apply_log (v_of lca) l1 == (v_of s1) /\ apply_log (v_of lca) l2 == (v_of s2)))
+          (ensures (eq (concrete_merge (v_of lca) (v_of s1) (v_of s2)) 
+                       (concrete_merge (v_of lca) (v_of s2) (v_of s1)))) = ()
+                       
 let linearizable_s1_0''_base_base (lca s1 s2':st) (last2:op_t)
   : Lemma (requires consistent_branches lca s1 s2' /\
                     is_prefix (ops_of lca) (snoc (ops_of s2') last2) /\
@@ -96,47 +102,6 @@ let linearizable_s1_0_s2_0_base (lca s1 s2:st)
         
           (ensures eq (v_of lca) (concrete_merge (v_of lca) (v_of s1) (v_of s2))) = ()
 
-let linearizable_s2_0''_base_base (lca s1' s2:st) (last1:op_t)
-  : Lemma (requires consistent_branches lca s1' s2 /\
-                    is_prefix (ops_of lca) (snoc (ops_of s1') last1) /\
-                    ops_of s1' = ops_of lca /\ ops_of s2 = ops_of lca /\
-                    length (ops_of lca) = 0 /\
-                    (forall id. mem_id id (ops_of lca) ==> lt id (fst last1)))
-         
-          (ensures eq (do (v_of s1') last1) (concrete_merge (v_of lca) (do (v_of s1') last1) (v_of s2))) = ()
-
-let linearizable_s2_0''_base_ind (lca s1' s2:st) (last1:op_t)
-  : Lemma (requires consistent_branches lca s1' s2 /\
-                    is_prefix (ops_of lca) (snoc (ops_of s1') last1) /\
-                    ops_of s1' = ops_of lca /\ ops_of s2 = ops_of lca /\
-                    length (ops_of lca) > 0 /\
-                    (forall id. mem_id id (ops_of lca) ==> lt id (fst last1)) /\
-
-                    (let l' = inverse_st lca in
-                    let s1'' = inverse_st s1' in
-                    let s2' = inverse_st s2 in
-                    consistent_branches l' s1'' s2' /\
-                    is_prefix (ops_of l') (snoc (ops_of s1'') last1) /\
-                    ops_of s1'' = ops_of l' /\ ops_of s2' = ops_of l' /\
-                    eq (do (v_of s1'') last1) (concrete_merge (v_of l') (do (v_of s1'') last1) (v_of s2'))))
-
-          (ensures eq (do (v_of s1') last1) (concrete_merge (v_of lca) (do (v_of s1') last1) (v_of s2))) = ()
-          
-let linearizable_s2_0''_ind (lca s1' s2:st) (last1:op_t)
-  : Lemma (requires consistent_branches_s1_gt0 lca s1' s2 /\
-                    is_prefix (ops_of lca) (snoc (ops_of s1') last1) /\
-                    ops_of s2 = ops_of lca /\
-                    (forall id. mem_id id (ops_of lca) ==> lt id (fst last1)) /\
-
-                    (let inv1 = inverse_st s1' in
-                    consistent_branches lca inv1 s2 /\
-                    is_prefix (ops_of lca) (snoc (ops_of inv1) last1) /\
-                    (exists l1. (do (v_of inv1) last1 == apply_log (v_of lca) l1)) /\
-                    (exists l1. (do (v_of s1') last1 == apply_log (v_of lca) l1)) /\
-                    eq (do (v_of inv1) last1) (concrete_merge (v_of lca) (do (v_of inv1) last1) (v_of s2))))
-         
-          (ensures eq (do (v_of s1') last1) (concrete_merge (v_of lca) (do (v_of s1') last1) (v_of s2))) = ()
-
 let linearizable_gt0_base (lca s1 s2:st) (last1 last2:op_t)
   : Lemma (requires consistent_branches lca s1 s2 /\
                     ops_of s1 = ops_of lca /\ ops_of s2 = ops_of lca /\
@@ -146,10 +111,6 @@ let linearizable_gt0_base (lca s1 s2:st) (last1 last2:op_t)
          
           (ensures (First_then_second? (resolve_conflict last1 last2) ==>
                       (eq (do (concrete_merge (v_of lca) (v_of s1) (do (v_of s2) last2)) last1)
-                         (concrete_merge (v_of lca) (do (v_of s1) last1) (do (v_of s2) last2)))) /\
-
-                   (Second_then_first? (resolve_conflict last1 last2) ==>
-                      (eq (do (concrete_merge (v_of lca) (do (v_of s1) last1) (v_of s2)) last2)
                          (concrete_merge (v_of lca) (do (v_of s1) last1) (do (v_of s2) last2))))) = ()              
 
 let linearizable_gt0_ind (lca s1 s2:st) (last1 last2:op_t)
@@ -171,13 +132,6 @@ let linearizable_gt0_ind (lca s1 s2:st) (last1 last2:op_t)
                     eq (do (concrete_merge (v_of lca) (v_of s1) (do (v_of s2') last2)) last1)
                        (concrete_merge (v_of lca) (do (v_of s1) last1) (do (v_of s2') last2))) ==>
                     (eq (do (concrete_merge (v_of lca) (v_of s1) (do (v_of s2) last2)) last1)
-                        (concrete_merge (v_of lca) (do (v_of s1) last1) (do (v_of s2) last2)))) /\
-                          
-                   ((ops_of s1 = ops_of lca /\
-                    Second_then_first? (resolve_conflict last1 last2) /\
-                    eq (do (concrete_merge (v_of lca) (do (v_of s1) last1) (v_of s2')) last2)
-                       (concrete_merge (v_of lca) (do (v_of s1) last1) (do (v_of s2') last2))) ==>
-                    (eq (do (concrete_merge (v_of lca) (do (v_of s1) last1) (v_of s2)) last2)
                         (concrete_merge (v_of lca) (do (v_of s1) last1) (do (v_of s2) last2)))))) = ()
 
 let linearizable_gt0_ind1 (lca s1 s2:st) (last1 last2:op_t)
@@ -200,13 +154,7 @@ let linearizable_gt0_ind1 (lca s1 s2:st) (last1 last2:op_t)
                    eq (do (concrete_merge (v_of lca) (v_of s1') (do (v_of s2) last2)) last1)
                       (concrete_merge (v_of lca) (do (v_of s1') last1) (do (v_of s2) last2))) ==>
                    eq (do (concrete_merge (v_of lca) (v_of s1) (do (v_of s2) last2)) last1)
-                      (concrete_merge (v_of lca) (do (v_of s1) last1) (do (v_of s2) last2))) /\
-
-                   ((Second_then_first? (resolve_conflict last1 last2) /\
-                    eq (do (concrete_merge (v_of lca) (do (v_of s1') last1) (v_of s2)) last2)
-                       (concrete_merge (v_of lca) (do (v_of s1') last1) (do (v_of s2) last2)) ==>
-                    eq (do (concrete_merge (v_of lca) (do (v_of s1) last1) (v_of s2)) last2)
-                       (concrete_merge (v_of lca) (do (v_of s1) last1) (do (v_of s2) last2)))))) = () 
+                      (concrete_merge (v_of lca) (do (v_of s1) last1) (do (v_of s2) last2))))) = () 
                        
 ////////////////////////////////////////////////////////////////
 //// Sequential implementation //////
